theories/variable.v
@@ -3,63 +3,30 @@ From iris.algebra Require Import excl auth frac_auth gmap gset.
 From iris.base_logic.lib Require Export invariants.
 From iris.program_logic Require Export atomic.
 From iris.heap_lang Require Import proofmode notation par.
-
-Class histG Σ := HistG {
-  hist_inG :> inG Σ (frac_authR (gmapUR nat (exclR valO)));
-  timestamp_inG :> inG Σ (exclR natO)
-}.
-Definition histΣ : gFunctors :=
-  #[GFunctor (frac_authR (gmapUR nat (exclR valO))); GFunctor (exclR natO)].
-Instance subG_histΣ {Σ} : subG histΣ Σ → histG Σ.
-Proof. solve_inG. Qed.
+From play Require Import history.
 
 Section var.
-  Context `{!heapG Σ} `{histG Σ} (N : namespace).
+  Context `{!heapG Σ} `{!@histG valO Σ} (N : namespace).
 
   Definition new : val := λ: "v", ref "v".
   Definition set : val := λ: "l" "x", "l" <- "x".
 
-  Definition last_op (t : nat) v (hs : gmapUR nat (exclR valO)) : iProp Σ :=
-    ⌜(∀ (t' : nat), (t' ∈ (dom (gset nat) hs) → t' ≤ t))
-    ∧ hs !! t = Some (Excl v) ⌝.
+  Definition is_hist l γh := inv N (∃ hs t v, (l ↦ v) ∗ hist γh hs t v).
 
-  Definition is_hist l γh γt :=
-    inv N (∃ v, (l ↦ v) ∗
-                (∃ hs (t : nat),
-                    own γh (●F hs) ∗
-                    own γt (Excl t) ∗
-                    last_op t v hs)).
-
-  Lemma set_spec (l : loc) (γh γt : gname) (q : Qp) (v : val) :
-    is_hist l γh γt -∗
-    <<< ∀ hs, own γh (◯F{q} hs) >>>
+  Lemma set_spec (l : loc) (γh : gname) (q : Qp) (v : val) :
+    is_hist l γh -∗
+    <<< ∀ hs, hist_snap γh q hs >>>
       set #l v @ ⊤ ∖ ↑N
-    <<< ∃ (t : nat),
-        own γh (◯F{q} (<[t := Excl v]> hs)),
-        RET #() >>>.
+    <<< ∃ (t : nat), hist_snap γh q (<[t := Excl v]> hs), RET #() >>>.
   Proof.
     iIntros "#Hist" (Φ) "AU". wp_lam; wp_let.
-    iInv N as (v') ">[Hl H]".
-    iDestruct "H" as (hsM tM) "[H● [Ht [% _]]]". rename H0 into tM_max.
+    iInv N as (hsM t v') "[Hl H]".
     iMod "AU" as (hs) "[H◯ [_ Hclose]]".
-    iMod (own_update with "Ht") as "Ht";
-      first by apply (cmra_update_exclusive (Excl (S tM))).
-    iMod (own_update_2 with "H● H◯") as "[H● H◯]".
-    { apply frac_auth_update, (alloc_local_update _ _ (S tM) (Excl v)); last done.
-      rewrite <-(not_elem_of_dom (D:=gset nat)).
-      intro. apply tM_max in H0. lia. }
-    wp_store. clear v'.
+    wp_store.
+    iMod (hist_update with "H H◯") as "[H H◯]".
     iMod ("Hclose" with "[H◯]") as "$"; first done.
     iModIntro; iModIntro; iNext.
-    iExists v. iSplitL "Hl"; first done.
-    iExists (<[S tM:=Excl v]> hsM), (S tM). iFrame.
-    iPureIntro. split; last by rewrite lookup_insert.
-    intros t'.
-    rewrite (dom_insert (M:=gmap nat) (D:=gset nat) (A:=excl valO)).
-    rewrite elem_of_union elem_of_singleton.
-    intro Ht'.
-    destruct Ht' as [Ht'|Ht'].
-    - by rewrite Ht'.
-    - apply tM_max in Ht'. lia.
+    iExists (<[S t:=Excl v]> hsM), (S t), v.
+    iFrame.
   Qed.
 End var.
