theories/history.v
@@ -1,0 +1,80 @@
+From iris.proofmode Require Import tactics.
+From iris.algebra Require Export excl auth frac_auth gmap gset updates local_updates.
+From iris.base_logic Require Export base_logic lib.own.
+
+(* snapshot history *)
+Section History.
+  Context {A : ofeT}.
+  Notation Hist := (gmapUR nat (exclR A)).
+
+  Class histG Σ := HistG { hist_inG :> inG Σ (frac_authR Hist) }.
+
+  Definition histΣ : gFunctors := #[GFunctor (frac_authR Hist)].
+
+  Instance subG_histΣ {Σ} : subG histΣ Σ → histG Σ.
+  Proof. solve_inG. Qed.
+
+  Context `{!histG Σ}.
+
+  (* init with <[0 := ...]> *)
+  Definition last_op (t : nat) a (hs : Hist) :=
+    (size hs = (S t)) ∧
+    (∀ t', t' ∈ (dom (gset nat) hs) → t' ≤ t) ∧
+    hs !! t = Some (Excl a).
+
+  Definition hist γh (hs : Hist) t a : iProp Σ :=
+    own γh (●F hs) ∗ ⌜last_op t a hs⌝.
+
+  Definition hist_snap γh q (hs : Hist) : iProp Σ := own γh (◯F{q} hs).
+
+  Lemma new_timestamp t a hs : last_op t a hs -> hs !! (S t) = None.
+  Proof.
+    intros (_ & Hmax & _).
+    rewrite -(not_elem_of_dom (D:=gset nat)) => H.
+    specialize (Hmax (S t) H).
+    lia.
+  Qed.
+
+  Lemma new_op (t : nat) a b (hs : Hist) :
+    last_op t a hs -> last_op (S t) b (<[S t := Excl b]> hs).
+  Proof.
+    intros (Hsize & Hmax & ?).
+    split; [|split]; last by rewrite lookup_insert.
+    - rewrite <-Hsize. apply: map_size_insert. rewrite Hsize.
+      by apply: new_timestamp.
+    - intros t'.
+      rewrite dom_insert elem_of_union elem_of_singleton => [[/ltac:(lia)|Ht']].
+      specialize (Hmax t' Ht'). lia.
+  Qed.
+
+  Lemma hist_update γh q (hsM hs : Hist) t a b :
+    hist γh hsM t a -∗ hist_snap γh q hs ==∗
+         hist γh (<[S t:=Excl b]> hsM) (S t) b ∗ hist_snap γh q (<[S t:=Excl b]> hs).
+  Proof.
+    rewrite /hist /hist_snap.
+    iIntros "[H● %] H◯ ".
+    iMod (own_update_2 with "H● H◯") as "[H● H◯]".
+    { apply frac_auth_update, (alloc_local_update _ _ (S t) (Excl b)); last done.
+      by apply: new_timestamp. }
+    iFrame; iModIntro; iPureIntro. by apply: new_op.
+  Qed.
+
+  (* NOTE Timeless requires {!OfeDiscrete A}  *)
+End History.
+Typeclasses Opaque hist hist_snap.
+
+(* TODO: snapshot before/after. TODO: vs operation history *)
+Section History2.
+  Context {A : ofeT}.
+  Notation Hist2 := (gmapUR nat (exclR (prodO A A))).
+
+  Class hist2G Σ := Hist2G { hist2_inG :> inG Σ (frac_authR Hist2) }.
+
+  Definition hist2Σ : gFunctors := #[GFunctor (frac_authR Hist2)].
+
+  Instance subG_hist2Σ {Σ} : subG hist2Σ Σ → hist2G Σ.
+  Proof. solve_inG. Qed.
+
+  (* TODO: well-formed *)
+
+End History2.
